revising the lemmas in Crypto.AEAD.PRF_MAC substantially ... setting up towards integration with Crypto.AEAD.Encrypt

examples/low-level/crypto/Crypto.AEAD.Encrypt.fst
@@ -163,7 +163,7 @@ let encrypt_write_effect i st n #aadlen aad #plainlen plain cipher_tag ak acc
   BufferUtils.chain_mods_enc abuf (not (safeMac i)) st.log_region PRF.(st.prf.mac_rgn) cipher_tag
 			     h_init h_push h_prf h_enx h_acc h_mac h_ideal
 
-assume val reestablish_inv:
+val reestablish_inv:
           i: id -> 
          st: aead_state i Writer ->
           n: Cipher.iv (alg i) ->
@@ -181,7 +181,7 @@ assume val reestablish_inv:
          h4: mem ->               
       Lemma 
   (requires  (let cipher : lbuffer (v plainlen) = Buffer.sub cipher_tag 0ul plainlen in
-              let x_1 = {iv=n; ctr=otp_offset i} in
+              (* let x_1 = {iv=n; ctr=otp_offset i} in *)
               enc_dec_separation st aad plain cipher_tag  /\
               enc_dec_liveness st aad plain cipher_tag h0 /\
               (* enc_dec_liveness st aad plain cipher_tag h1 /\ *)
@@ -190,14 +190,23 @@ assume val reestablish_inv:
 	      HS.(is_stack_region h0.tip) /\ //TODO: need to add that the buffers of acc live in h0.tip
               inv st h0 /\
 	      (safeMac i ==> is_mac_for_iv st ak h0) /\
-              Enxor.enxor_invariant st.prf x_1 plainlen 0ul plain cipher h0 h1 /\
-              Enxor.modifies_table_above_x_and_buffer st.prf x_1 cipher h0 h1 /\
+              PRF_MAC.enxor_h0_h1 st n aad plain cipher_tag h0 h1 /\
+              (* Enxor.enxor_invariant st.prf x_1 plainlen 0ul plain cipher h0 h1 /\ *)
+              (* Enxor.modifies_table_above_x_and_buffer st.prf x_1 cipher h0 h1 /\ *)
               EncodingWrapper.accumulate_modifies_nothing h1 h2 /\
               CMAWrapper.mac_ensures i n st aad plain cipher_tag ak acc h2 h3 /\ (
               if safeMac i
               then ideal_ensures st n aad plain cipher_tag h3 h4
               else h3 == h4)))
   (ensures    (inv st h4))
+let reestablish_inv i st n #aadlen aad #plainlen plain cipher_tag ak acc h0 h1 h2 h3 h4 =
+  let cipher : lbuffer (v plainlen) = Buffer.sub cipher_tag 0ul plainlen in
+  PRF_MAC.lemma_propagate_inv_enxor st n aad plain cipher_tag h0 h1;
+  (* assert (PRF_MAC.enxor_post st n aad plain cipher h1); *)
+  FStar.Buffer.lemma_intro_modifies_0 h1 h2;
+  (* assert (PRF_MAC.accumulate_h0_h1 st n aad plain cipher h1 h2); *)
+  PRF_MAC.lemma_propagate_inv_accumulate false st n aad plain cipher_tag h1 h2;
+  admit()
 
 ////////////////////////////////////////////////////////////////////////////////
        
@@ -220,13 +229,6 @@ val encrypt:
 	      encrypt_ensures st n aad plain cipher_tag h0 h1 /\
 	      encrypt_modifies st cipher_tag h0 h1 /\
  	      inv st h1))
-
-assume val frame_inv_pop (#i:id) (#rw:rw) (st:aead_state i rw) (h:mem)
-   : Lemma (inv st h /\ 
-	    HS.poppable h ==> inv st (HS.pop h))
-	    
-   (* = if safeMac i *)
-   (*   then frame_refines i st.prf.mac_rgn (HS.sel h (PRF.itable i st.prf)) (HS.sel h st.log) h h1 *)
 
 let encrypt i st n aadlen aad plainlen plain cipher_tagged =
   let h_init = get() in
