examples/low-level/crypto/Crypto.AEAD.Invariant.fst
@@ -509,6 +509,12 @@ let frame_inv_push (#i:id) (#rw:rw) (st:aead_state i rw) (h:mem) (h1:mem)
    = if safeMac i
      then frame_refines i st.prf.mac_rgn (HS.sel h (PRF.itable i st.prf)) (HS.sel h st.log) h h1
 
+let frame_inv_pop (#i:id) (#rw:rw) (st:aead_state i rw) (h:mem{HS.poppable h})
+   : Lemma (requires (inv st h))
+	   (ensures  (inv st (HS.pop h)))
+   = if safeMac i
+     then frame_refines i st.prf.mac_rgn (HS.sel h (PRF.itable i st.prf)) (HS.sel h st.log) h (HS.pop h)
+
 let weaken_all_above (#rgn:region) (#i:id) (s:Seq.seq (PRF.entry rgn i)) 
 		    (x:PRF.domain i) (y:PRF.domain i{y `above` x})
     : Lemma (all_above y s ==> all_above x s)
